Launchbury/CoCallFix.thy
@@ -1,0 +1,107 @@
+theory CoCallFix
+imports CoCallAnalysis ArityAnalysisFix
+begin
+
+locale CoCallArityAnalysis = CoCallAnalysis + ArityAnalysis
+
+context CoCallArityAnalysis
+begin
+
+definition ccBind :: "var \<Rightarrow> exp \<Rightarrow> ((AEnv \<times> CoCalls) \<rightarrow> CoCalls)"
+  where "ccBind v e = (\<Lambda> (ae, G).  if (v--v\<notin>G) \<or> \<not> isLam e then cc_restr (fv e) (ccExp' e \<cdot> (ae v)) else ccSquare (fv e))"
+(* paper has:  \<or> ae v = up\<cdot>0, but that is not monotone! But should give the same result. *)
+
+lemma ccBind_eq[simp]: "ccBind v e \<cdot> (ae, G) = (if (v--v\<notin>G) \<or> \<not> isLam e then cc_restr (fv e) (ccExp' e \<cdot> (ae v)) else ccSquare (fv e))"
+  unfolding ccBind_def
+  apply (rule cfun_beta_Pair)
+  apply (rule cont_if_else_above)
+  apply simp
+  apply simp
+  apply (auto dest: set_mp[OF ccFieldd_cc_restr])[1]
+  (* Abstraction broken! Fix this. *)
+  apply (case_tac p, auto, transfer, auto)[1]
+  apply (rule adm_subst[OF cont_snd])
+  apply (rule admI, thin_tac "chain ?x", transfer, auto)
+  done
+
+lemma ccBind_strict[simp]: "ccBind v e \<cdot> \<bottom> = \<bottom>"
+  by (auto simp add: inst_prod_pcpo simp del: Pair_strict)
+
+fun ccBinds :: "heap \<Rightarrow> ((AEnv \<times> CoCalls) \<rightarrow> CoCalls)"
+  where "ccBinds [] = csnd"
+     |  "ccBinds ((v,e)#binds) = ccBind v e \<squnion> ccBinds (delete v binds)"
+
+lemma ccBinds_strict[simp]: "ccBinds \<Gamma>\<cdot>\<bottom>=\<bottom>"
+  by (induct \<Gamma> rule: ccBinds.induct) auto
+
+lemma ccBinds_strict'[simp]: "ccBinds \<Gamma>\<cdot>(\<bottom>,\<bottom>)=\<bottom>"
+  by (induct \<Gamma> rule: ccBinds.induct) auto
+
+lemma ccBinds_reorder1: "map_of \<Gamma> v = Some e \<Longrightarrow> ccBinds \<Gamma> = ccBind v e \<squnion> ccBinds (delete v \<Gamma>)"
+proof (induction \<Gamma> rule: ccBinds.induct)
+  case 1 thus ?case by simp
+next
+  case (2 v' e' \<Gamma>)
+  thus ?case
+  apply (cases "v' = v")
+  apply auto
+  apply (metis (hide_lams, no_types) join_assoc delete_twist join_comm)
+  done
+qed
+
+definition ccBindsExtra :: "heap \<Rightarrow> ((AEnv \<times> CoCalls) \<rightarrow> CoCalls)"
+  where "ccBindsExtra \<Gamma> = (\<Lambda> i.  ccBinds \<Gamma> \<cdot> i \<squnion> ccProd (fv \<Gamma> - domA \<Gamma>) (ccNeighbors (domA \<Gamma>) (ccBinds \<Gamma> \<cdot> i)))"
+
+lemma ccBindsExtra_simp: "ccBindsExtra \<Gamma> \<cdot> i = ccBinds \<Gamma> \<cdot> i \<squnion> ccProd (fv \<Gamma> - domA \<Gamma>) (ccNeighbors (domA \<Gamma>) (ccBinds \<Gamma> \<cdot> i))"
+  unfolding ccBindsExtra_def by simp
+
+lemma ccBindsExtra_strict[simp]: "ccBindsExtra \<Gamma> \<cdot> \<bottom> = \<bottom>"
+  by (auto simp add: ccBindsExtra_simp inst_prod_pcpo simp del: Pair_strict)
+
+definition ccFix ::  "heap \<Rightarrow> ((AEnv \<times> CoCalls) \<rightarrow> (AEnv \<times> CoCalls))"
+  where "ccFix \<Gamma> = (\<Lambda> i. (\<mu>  i'. (ABinds \<Gamma> \<cdot> (fst i'), ccBindsExtra \<Gamma> \<cdot> i') \<squnion> i))"
+
+lemma ccFix_eq: "ccFix \<Gamma> \<cdot> i = (\<mu>  i'. (ABinds \<Gamma> \<cdot> (fst i'), ccBindsExtra \<Gamma> \<cdot> i') \<squnion> i)"
+  unfolding ccFix_def by simp
+
+lemma ccFix_strict[simp]: "ccFix \<Gamma> \<cdot> \<bottom> = \<bottom>"
+  unfolding ccFix_eq
+  by (rule fix_eqI) auto
+
+(*
+lemma ccFix_least_below: "Binds \<Gamma> \<cdot> (fst ae') \<sqsubseteq> fst ae' \<Longrightarrow> ae \<sqsubseteq> ae' \<Longrightarrow> ccFix \<Gamma> \<cdot> ae \<sqsubseteq> ae'"
+  unfolding ccFix_eq
+  by (auto intro: fix_least_below)
+
+lemma Afix_unroll: "Afix \<Gamma>\<cdot>ae = ABinds \<Gamma> \<cdot> (Afix \<Gamma>\<cdot>ae) \<squnion> ae"
+  unfolding Afix_eq
+  apply (subst fix_eq)
+  by simp
+
+lemma Abinds_below_Afix: "ABinds \<Delta> \<sqsubseteq> Afix \<Delta>"
+  apply (rule cfun_belowI)
+  apply (simp add: Afix_eq)
+  apply (subst fix_eq, simp)
+  apply (rule below_trans[OF _ join_above1])
+  apply (rule monofun_cfun_arg)
+  apply (subst fix_eq, simp)
+  done
+
+lemma Afix_above_arg: "ae \<sqsubseteq> Afix \<Gamma> \<cdot> ae"
+  by (metis (hide_lams, no_types) Abinds_below_Afix ArityAnalysis.ABinds_above_arg below_refl box_below monofun_cfun_fun)
+
+
+lemma Abinds_Afix[simp]: "ABinds \<Gamma>\<cdot>(Afix \<Gamma>\<cdot>ae) = Afix \<Gamma>\<cdot>ae"
+  unfolding Afix_eq
+  apply (subst fix_eq) back apply simp
+  apply (rule below_trans[OF ABinds_above_arg monofun_cfun_arg])
+  apply (subst fix_eq) apply simp
+  done
+
+lemma Afix_reorder: "map_of \<Gamma> = map_of \<Delta> \<Longrightarrow> Afix \<Gamma> = Afix \<Delta>"
+  by (intro cfun_eqI)(simp add: Afix_eq cong: Abinds_reorder)
+*)
+
+end
+
+end
