Launchbury/CoCallGraph-Nominal.thy
@@ -1,0 +1,25 @@
+theory "CoCallGraph-Nominal"
+imports CoCallGraph "Nominal-HOLCF"
+begin
+
+instantiation CoCalls :: pt
+begin
+  lift_definition permute_CoCalls :: "perm \<Rightarrow> CoCalls \<Rightarrow> CoCalls" is "permute".
+instance
+  apply default
+  apply (transfer, simp)+
+  done
+end
+
+instance CoCalls :: cont_pt
+  apply default
+  apply (rule contI2)
+  apply (rule monofunI)
+  apply transfer
+  apply (metis (full_types) True_eqvt subset_eqvt)
+  apply (thin_tac "chain ?x")+
+  apply transfer
+  apply simp
+  done  
+
+end
