Launchbury/CoCallGraph.thy
@@ -1,5 +1,5 @@
 theory CoCallGraph
-imports Main Vars HOLCF
+imports Main Vars "HOLCF-Join-Classes"
 begin
 
 typedef CoCalls = "UNIV :: (var \<times> var) set set"
@@ -47,6 +47,38 @@ proof-
   show ?thesis by metis
 qed
 
+lift_definition is_cc_lub :: "CoCalls set \<Rightarrow> CoCalls \<Rightarrow> bool" is "(\<lambda> S x . x = Union S)".
+print_theorems
+
+lemma ccis_lubTransfer[transfer_rule]: "(rel_set pcr_CoCalls  ===> pcr_CoCalls ===> op =) (\<lambda> S x . x = Union S) op <<|"
+proof-
+  have "is_cc_lub = op <<|"
+  apply (rule, rule, rule)
+  unfolding is_lub_def is_ub_def
+  apply transfer
+  apply auto
+  unfolding is_lub_def is_ub_def
+  apply transfer
+  apply blast
+  done
+  thus ?thesis using is_cc_lub.transfer by simp
+qed
+
+lift_definition ccEmpty :: "CoCalls" is "{}".
+
+instance CoCalls :: pcpo
+proof default
+  have "\<forall>y . ccEmpty \<sqsubseteq> y" by transfer simp
+  thus "\<exists>x. \<forall>y. (x::CoCalls) \<sqsubseteq> y"..
+qed
+
+lemma ccBotTransfer[transfer_rule]: "pcr_CoCalls {} \<bottom>"
+proof-
+  have "\<And>x. ccEmpty \<sqsubseteq> x" by transfer simp
+  hence "ccEmpty = \<bottom>" by (rule bottomI)
+  thus ?thesis using ccEmpty.transfer by simp
+qed
+
 lift_definition ccField :: "CoCalls \<Rightarrow> var set" is Field.
 
 lift_definition inCC :: "var \<Rightarrow> var \<Rightarrow> CoCalls \<Rightarrow> bool" ("_--_\<in>_")
@@ -54,6 +86,9 @@ lift_definition inCC :: "var \<Rightarrow> var \<Rightarrow> CoCalls \<Rightarro
 
 abbreviation notInCC :: "var \<Rightarrow> var \<Rightarrow> CoCalls \<Rightarrow> bool" ("_--_\<notin>_")
   where "x--y\<notin>S \<equiv> \<not> (x--y\<in>S)"
+
+lemma notInCC_bot[simp]: "(x--y\<in>\<bottom>) \<longleftrightarrow> False"
+  by transfer auto
 
 lift_definition cc_delete :: "var \<Rightarrow> CoCalls \<Rightarrow> CoCalls"
   is "\<lambda> z. Set.filter (\<lambda> (x,y) . x \<noteq> z \<and> y \<noteq> z)".
@@ -64,6 +99,60 @@ lemma ccField_cc_delete: "ccField (cc_delete x S) \<subseteq> ccField S - {x}"
 lift_definition ccProd :: "var set \<Rightarrow> var set \<Rightarrow> CoCalls"
   is "\<lambda> S1 S2. S1 \<times> S2 \<union> S2 \<times> S1".
 
+lemma ccProd_empty[simp]: "ccProd {} S = \<bottom>" by transfer auto
+
+lemma ccProd_empty'[simp]: "ccProd S {} = \<bottom>" by transfer auto
+
+
+lift_definition cc_restr :: "var set \<Rightarrow> CoCalls \<Rightarrow> CoCalls"
+  is "\<lambda> S. Set.filter (\<lambda> (x,y) . x \<in> S \<and> y \<in> S)".
+
+lemma ccFieldd_cc_restr: "ccField (cc_restr S G) \<subseteq> ccField G \<inter> S"
+  by transfer (auto simp add: Field_def)
+
+lemma cc_restr_bot[simp]: "cc_restr S \<bottom> = \<bottom>"
+  by transfer auto
+
+lemma cont_cc_restr: "cont (cc_restr S)"
+  apply (rule contI)
+  apply (thin_tac "chain ?x")
+  apply transfer
+  apply auto
+  done
+
+lemmas cont_compose[OF cont_cc_restr, cont2cont, simp]
+
 definition ccSquare where "ccSquare S = ccProd S S"
+
+lemma ccField_ccSquare[simp]: "ccField (ccSquare S) = S"
+  unfolding ccSquare_def by transfer (auto simp add: Field_def)
+  
+lemma below_ccSquare[iff]: "G \<sqsubseteq> ccSquare S  \<longleftrightarrow> ccField G \<subseteq> S"
+  unfolding ccSquare_def by transfer (auto simp add: Field_def)
+
+lift_definition ccNeighbors :: "var set \<Rightarrow> CoCalls \<Rightarrow> var set" 
+  is "\<lambda> S G. {y . \<exists> x \<in> S. (y,x) \<in> G \<or> (x,y) \<in> G}".
+
+lemma ccNeighbors_bot[simp]: "ccNeighbors S \<bottom> = {}" by transfer auto
+
+lemma cont_ccProd_ccNeighbors:
+  "cont (\<lambda>x. ccProd S (ccNeighbors S' x))"
+  apply (rule contI)
+  apply (thin_tac "chain ?x")
+  apply transfer
+  apply auto
+  done
+
+lemmas cont_compose[OF cont_ccProd_ccNeighbors, cont2cont]
+
+instance CoCalls :: Finite_Join_cpo
+proof default
+  fix x y :: CoCalls
+  show "compatible x y"
+    unfolding compatible_def
+    apply (rule exI)
+    apply (rule coCallsLub_is_lub)
+    done
+qed
 
 end
